systems/SeqNum.v
@@ -4,8 +4,7 @@ Set Implicit Arguments.
 
 Section SeqNum.
   Context {orig_base_params : BaseParams}.
-  Context {orig_name_params : NameParams}.
-  Context {orig_multi_params : MultiParams orig_base_params orig_name_params}.
+  Context {orig_multi_params : MultiParams orig_base_params}.
 
   Record seq_num_data := mkseq_num_data { tdNum  : nat;
                             tdSeen : name -> list nat;
@@ -60,27 +59,22 @@ Section SeqNum.
       output := output
     }.
 
-  Instance name_params : NameParams :=
+  Instance multi_params : MultiParams _ :=
     {
       name := name ;
+      msg := seq_num_msg ;
+      msg_eq_dec := seq_num_msg_eq_dec ;
       name_eq_dec := name_eq_dec ;
-      nodes := nodes
+      nodes := nodes ;
+      init_handlers := seq_num_init_handlers;
+      net_handlers := seq_num_net_handlers;
+      input_handlers := seq_num_input_handlers
     }.
   Proof.
     - eauto using all_names_nodes.
     - eauto using no_dup_nodes.
   Defined.
-
-  Instance multi_params : MultiParams _ _ :=
-    {      
-      msg := seq_num_msg ;
-      msg_eq_dec := seq_num_msg_eq_dec ;            
-      init_handlers := seq_num_init_handlers;
-      net_handlers := seq_num_net_handlers;
-      input_handlers := seq_num_input_handlers
-    }.
 End SeqNum.
 
 Hint Extern 5 (@BaseParams) => apply base_params : typeclass_instances.
-Hint Extern 5 (@NameParams) => apply name_params : typeclass_instances.
-Hint Extern 5 (@MultiParams _ _) => apply multi_params : typeclass_instances.
+Hint Extern 5 (@MultiParams _) => apply multi_params : typeclass_instances.
